Proof for HonestReplicasLockOnCommitForGivenView verified.

proof.dfy
@@ -18,6 +18,12 @@ module Proof {
   import opened SafetySpec
   import Library
 
+  predicate IsHonestReplica(c:Constants, hostId:HostId) 
+  {
+    && c.WF()
+    && c.IsReplica(hostId)
+  }
+
   // Here's a predicate that will be very useful in constructing inviariant conjuncts.
   predicate RecordedPrePreparesRecvdCameFromNetwork(c:Constants, v:Variables) {
     && v.WF(c)
@@ -51,7 +57,7 @@ module Proof {
   predicate EveryCommitMsgIsSupportedByAQuorumOfPrepares(c:Constants, v:Variables) {
     && v.WF(c)
     && (forall commitMsg | commitMsg in v.network.sentMsgs && commitMsg.Commit? ::
-          QuorumOfPreparesInNetwork(c, v, commitMsg.seqID) )
+          QuorumOfPreparesInNetwork(c, v, commitMsg.seqID, commitMsg.clientOp) )
   }
 
   predicate HonestReplicasLockOnCommitForGivenView(c:Constants, v:Variables) {
@@ -60,33 +66,86 @@ module Proof {
         && msg2 in v.network.sentMsgs 
         && msg1.Commit?
         && msg2.Commit?
+        && msg1.view == msg2.view
         && msg1.seqID == msg2.seqID
         && msg1.sender == msg2.sender
+        && IsHonestReplica(c, msg1.sender)
         :: msg1 == msg2)
   }
 
+  predicate RecordedPreparesClientOpsMatchPrePrepare(c:Constants, v:Variables) {
+    && v.WF(c)
+    && (forall replicaIdx, seqID, sender |
+          && c.IsReplica(replicaIdx)
+          && var prepareMap := v.hosts[replicaIdx].replicaVariables.workingWindow.preparesRcvd;
+          && seqID in prepareMap
+          && sender in prepareMap[seqID]
+          :: && v.hosts[replicaIdx].replicaVariables.workingWindow.prePreparesRcvd[seqID].Some?         
+             && v.hosts[replicaIdx].replicaVariables.workingWindow.preparesRcvd[seqID][sender].clientOp 
+             == v.hosts[replicaIdx].replicaVariables.workingWindow.prePreparesRcvd[seqID].value.clientOp)
+  }
+
+  predicate RecordedCommitsClientOpsMatchPrePrepare(c:Constants, v:Variables) {
+    && v.WF(c)
+    && (forall replicaIdx, seqID, sender |
+          && c.IsReplica(replicaIdx)
+          && var commitMap := v.hosts[replicaIdx].replicaVariables.workingWindow.commitsRcvd;
+          && seqID in commitMap
+          && sender in commitMap[seqID]
+          :: && v.hosts[replicaIdx].replicaVariables.workingWindow.prePreparesRcvd[seqID].Some?
+             && v.hosts[replicaIdx].replicaVariables.workingWindow.commitsRcvd[seqID][sender].clientOp 
+             == v.hosts[replicaIdx].replicaVariables.workingWindow.prePreparesRcvd[seqID].value.clientOp)
+  }
+
+  predicate EveryCommitIsSupportedByRecordedPrepares(c:Constants, v:Variables) {
+    && v.WF(c)
+    && (forall commitMsg | && commitMsg in v.network.sentMsgs
+                           && commitMsg.Commit?
+                           && IsHonestReplica(c, commitMsg.sender)
+          :: && Replica.QuorumOfPrepares(c.hosts[commitMsg.sender].replicaConstants, 
+                                         v.hosts[commitMsg.sender].replicaVariables, 
+                                         commitMsg.seqID))
+  }
+
+  predicate EveryCommitClientOpMatchesRecordedPrePrepare(c:Constants, v:Variables) {
+    && v.WF(c)
+    && (forall commitMsg | && commitMsg in v.network.sentMsgs
+                           && commitMsg.Commit?
+                           && IsHonestReplica(c, commitMsg.sender)
+          :: && var recordedPrePrepare := 
+                v.hosts[commitMsg.sender].replicaVariables.workingWindow.prePreparesRcvd[commitMsg.seqID]; 
+             && recordedPrePrepare.Some?
+             && commitMsg.clientOp == recordedPrePrepare.value.clientOp)
+  }
 
   predicate Inv(c: Constants, v:Variables) {
     && RecordedPrePreparesRecvdCameFromNetwork(c, v)
     && RecordedPreparesInAllHostsRecvdCameFromNetwork(c, v)
     && EveryCommitMsgIsSupportedByAQuorumOfPrepares(c, v)
-    //&& HonestReplicasLockOnCommitForGivenView(c, v)
+    && RecordedPreparesClientOpsMatchPrePrepare(c, v)
+    && RecordedCommitsClientOpsMatchPrePrepare(c, v)
+    && EveryCommitIsSupportedByRecordedPrepares(c, v)
+    && EveryCommitClientOpMatchesRecordedPrePrepare(c, v)
+    && HonestReplicasLockOnCommitForGivenView(c, v)
   }
 
-  function sentPreparesForSeqID(c: Constants, v:Variables, seqID:Messages.SequenceID) : set<Messages.Message> 
+  function sentPreparesForSeqID(c: Constants, v:Variables, seqID:Messages.SequenceID,
+                                  clientOp:Messages.ClientOperation) : set<Messages.Message> 
   {
     set msg | && msg in v.network.sentMsgs 
               && msg.Prepare?
               && msg.seqID == seqID
+              && msg.clientOp == clientOp
   }
 
   function sendersOf(msgs:set<Messages.Message>) : set<HostIdentifiers.HostId> {
     set msg | msg in msgs :: msg.sender
   }
 
-  predicate QuorumOfPreparesInNetwork(c:Constants, v:Variables, seqID:Messages.SequenceID) {
+  predicate QuorumOfPreparesInNetwork(c:Constants, v:Variables, seqID:Messages.SequenceID, 
+                                      clientOp:Messages.ClientOperation) {
     && v.WF(c)
-    && var prepares := sentPreparesForSeqID(c, v, seqID);
+    && var prepares := sentPreparesForSeqID(c, v, seqID, clientOp);
     && |sendersOf(prepares)| >= c.clusterConfig.AgreementQuorum()
     //&& (forall prepare | prepare in prepares :: prepare.clientOp == clientOperation)
   }
@@ -103,14 +162,14 @@ module Proof {
              var h_v := v.hosts[step.id].replicaVariables;
              var h_v' := v'.hosts[step.id].replicaVariables;
              Replica.NextStep(h_c, h_v, h_v', step.msgOps, h_step)
-    ensures (forall seqID | QuorumOfPreparesInNetwork(c, v, seqID)
-                                        :: QuorumOfPreparesInNetwork(c, v', seqID))
+    ensures (forall seqID, clientOp | QuorumOfPreparesInNetwork(c, v, seqID, clientOp)
+                                        :: QuorumOfPreparesInNetwork(c, v', seqID, clientOp))
   {
-    forall seqID | QuorumOfPreparesInNetwork(c, v, seqID)
-                                  ensures QuorumOfPreparesInNetwork(c, v', seqID)
+    forall seqID, clientOp | QuorumOfPreparesInNetwork(c, v, seqID, clientOp)
+                                  ensures QuorumOfPreparesInNetwork(c, v', seqID, clientOp)
     {
-      var senders := sendersOf(sentPreparesForSeqID(c, v, seqID));
-      var senders' := sendersOf(sentPreparesForSeqID(c, v', seqID));
+      var senders := sendersOf(sentPreparesForSeqID(c, v, seqID, clientOp));
+      var senders' := sendersOf(sentPreparesForSeqID(c, v', seqID, clientOp));
       Library.SubsetCardinality(senders, senders');
     }
   }
@@ -123,15 +182,15 @@ module Proof {
     // A proof of EveryCommitMsgIsSupportedByAQuorumOfPrepares,
     // by selecting an arbitrary commitMsg instance
     forall commitMsg | commitMsg in v'.network.sentMsgs && commitMsg.Commit? ensures 
-      QuorumOfPreparesInNetwork(c, v', commitMsg.seqID) {
+      QuorumOfPreparesInNetwork(c, v', commitMsg.seqID, commitMsg.clientOp) {
       if(commitMsg in v.network.sentMsgs) { // the commitMsg has been sent in a previous step
         // In this case, the proof is trivial - we just need to "teach" Dafny about subset cardinality
-        var senders := sendersOf(sentPreparesForSeqID(c, v, commitMsg.seqID));
-        var senders' := sendersOf(sentPreparesForSeqID(c, v', commitMsg.seqID));
+        var senders := sendersOf(sentPreparesForSeqID(c, v, commitMsg.seqID, commitMsg.clientOp));
+        var senders' := sendersOf(sentPreparesForSeqID(c, v', commitMsg.seqID, commitMsg.clientOp));
         Library.SubsetCardinality(senders, senders');
       } else { // the commitMsg is being sent in the current step
-        var prepares := sentPreparesForSeqID(c, v, commitMsg.seqID);
-        var prepares' := sentPreparesForSeqID(c, v', commitMsg.seqID);
+        var prepares := sentPreparesForSeqID(c, v, commitMsg.seqID, commitMsg.clientOp);
+        var prepares' := sentPreparesForSeqID(c, v', commitMsg.seqID, commitMsg.clientOp);
         assert prepares == prepares'; // Trigger (hint) - sending a commitMsg does not affect the set of prepares
         
         // Prove that the prepares in the working window are a subset of the prepares in the network:
@@ -146,6 +205,99 @@ module Proof {
         Library.SubsetCardinality(prepareSendersInWorkingWindow, prepareSendersFromNetwork);
       }
     }
+  }
+
+  predicate ReplicaInternalMsg(msg:Messages.Message)
+  {
+    || msg.PrePrepare?
+    || msg.Prepare?
+    || msg.Commit?
+  }
+
+  lemma SendersAreAlwaysFewerThanMessages(msgs:set<Messages.Message>)
+    ensures |sendersOf(msgs)| <= |msgs|
+  {
+    if |msgs| > 0 {
+      var sender :| sender in sendersOf(msgs);
+      var msgsFromSender := set msg | && msg in msgs 
+                                      && msg.sender == sender;
+      var subMsgs := msgs - msgsFromSender;
+      SendersAreAlwaysFewerThanMessages(subMsgs);
+      Library.SubsetCardinality(sendersOf(subMsgs), sendersOf(msgs) - {sender});
+      assert sendersOf(msgs) - {sender} == sendersOf(subMsgs); // Trigger
+    }
+  }
+
+  lemma WlogCommitAgreement(c: Constants, v:Variables, v':Variables, step:Step, h_step:Replica.Step,
+                            old_msg:Messages.Message, new_msg:Messages.Message)
+    requires NextStep(c, v, v', step)
+    requires c.IsReplica(step.id)
+    requires  var h_c := c.hosts[step.id].replicaConstants;
+              var h_v := v.hosts[step.id].replicaVariables;
+              var h_v' := v'.hosts[step.id].replicaVariables;
+              && Replica.NextStep(h_c, h_v, h_v', step.msgOps, h_step)
+              && h_step.SendCommitStep?
+              && Replica.SendCommit(h_c, h_v, h_v', step.msgOps, h_step.seqID)
+    requires old_msg in v.network.sentMsgs && old_msg in v'.network.sentMsgs && ReplicaInternalMsg(old_msg)
+    requires new_msg !in v.network.sentMsgs && new_msg in v'.network.sentMsgs && ReplicaInternalMsg(new_msg)
+    requires && old_msg.seqID == new_msg.seqID
+             && old_msg.view == new_msg.view
+             && old_msg.sender == new_msg.sender
+             && old_msg.Commit?
+             && new_msg.Commit?
+
+    requires Inv(c, v)
+    ensures old_msg == new_msg
+  {
+    var h_c := c.hosts[step.id].replicaConstants;
+    var h_v := v.hosts[step.id].replicaVariables;
+    var h_v' := v'.hosts[step.id].replicaVariables;
+    QuorumOfPreparesInNetworkMonotonic(c, v, v', step, h_step);
+    assert QuorumOfPreparesInNetwork(c, v', old_msg.seqID, old_msg.clientOp);
+    assert Replica.QuorumOfPrepares(h_c, h_v, new_msg.seqID);
+    var recordedPreparesSenders := h_v.workingWindow.preparesRcvd[new_msg.seqID].Keys;
+    assert |recordedPreparesSenders| >= c.clusterConfig.AgreementQuorum();
+    var prepares := sentPreparesForSeqID(c, v, new_msg.seqID, new_msg.clientOp);
+    assert recordedPreparesSenders <= sendersOf(prepares) by {
+      forall sender | sender in recordedPreparesSenders ensures sender in sendersOf(prepares) {
+        var msg := h_v.workingWindow.preparesRcvd[new_msg.seqID][sender];
+        assert msg.sender == sender;
+        assert msg.seqID == new_msg.seqID;
+        assert msg.clientOp == new_msg.clientOp;
+        assert msg in v.network.sentMsgs;
+        assert msg in prepares;
+      }
+    }
+
+    var prepares' := sentPreparesForSeqID(c, v, new_msg.seqID, new_msg.clientOp);
+    Library.SubsetCardinality(prepares, prepares');
+
+    assert forall sender | sender in h_v.workingWindow.preparesRcvd[new_msg.seqID]
+                         :: h_v.workingWindow.preparesRcvd[new_msg.seqID][sender].clientOp == new_msg.clientOp;
+
+    assert h_v.workingWindow.prePreparesRcvd[new_msg.seqID].value.clientOp == new_msg.clientOp;
+
+    assert Replica.QuorumOfPrepares(h_c, h_v, old_msg.seqID);
+
+    assert h_v.workingWindow.prePreparesRcvd[old_msg.seqID].value.clientOp == old_msg.clientOp;
+
+    assert forall sender | sender in h_v.workingWindow.preparesRcvd[old_msg.seqID]
+                         :: h_v.workingWindow.preparesRcvd[old_msg.seqID][sender].clientOp == old_msg.clientOp;
+
+    Library.SubsetCardinality(recordedPreparesSenders, sendersOf(prepares));
+    assert |sendersOf(prepares)| >= c.clusterConfig.AgreementQuorum();
+    SendersAreAlwaysFewerThanMessages(prepares);
+    assert |prepares| >= |sendersOf(prepares)|;
+    assert |prepares| >= c.clusterConfig.AgreementQuorum();
+    assert QuorumOfPreparesInNetwork(c, v', new_msg.seqID, new_msg.clientOp);
+
+    assert old_msg.seqID == new_msg.seqID;
+    assert old_msg.Commit? && new_msg.Commit?;
+    assert old_msg.sender == new_msg.sender;
+    assert old_msg.view == new_msg.view;
+    assert old_msg.clientOp == new_msg.clientOp;
+
+    assert old_msg == new_msg;
   }
 
   lemma InvariantNext(c: Constants, v:Variables, v':Variables)
@@ -171,7 +323,34 @@ module Proof {
         case RecvPrePrepareStep => { assert Inv(c, v'); }
         case SendPrepareStep(seqID) => { assert Inv(c, v'); }
         case RecvPrepareStep => { assert Inv(c, v'); }
-        case SendCommitStep(seqID) => { assert Inv(c, v'); }
+        case SendCommitStep(seqID) => {
+          // HonestReplicasLockOnACommitForAGiveView
+          forall msg1, msg2 | 
+            && msg1 in v'.network.sentMsgs 
+            && msg2 in v'.network.sentMsgs 
+            && msg1.Commit?
+            && msg2.Commit?
+            && msg1.view == msg2.view
+            && msg1.seqID == msg2.seqID
+            && msg1.sender == msg2.sender
+            && IsHonestReplica(c, msg1.sender)
+            ensures msg1 == msg2 {
+              if(msg1 in v.network.sentMsgs && msg2 in v.network.sentMsgs) {
+                assert msg1 == msg2;
+              } else if(msg1 !in v.network.sentMsgs && msg2 !in v.network.sentMsgs) {
+                assert msg1 == msg2;
+              } else if(msg1 in v.network.sentMsgs && msg2 !in v.network.sentMsgs) {
+                WlogCommitAgreement(c, v, v', step, h_step, msg1, msg2);
+                assert msg1 == msg2;
+              } else if(msg1 !in v.network.sentMsgs && msg2 in v.network.sentMsgs) {
+                WlogCommitAgreement(c, v, v', step, h_step, msg2, msg1);
+                assert msg1 == msg2;
+              } else {
+                assert false;
+              }
+            }
+          assert Inv(c, v');
+        }
         case RecvCommitStep() => { assert Inv(c, v'); }
         case DoCommitStep(seqID) => { assert Inv(c, v'); }
     } else if (c.IsClient(step.id)) {
